[WIP] sigma and signatures are associative lists

theories/check.v
@@ -2,6 +2,22 @@ From mathcomp Require Import all_ssreflect.
 From det Require Import lang.
 From det Require Import tree tree_prop.
 
+(* TODO:
+A valid state for substitutions is mandatory?
+Given the following program execution
+(main X) => (p X, q X) => p X succeeds setting X to func, then
+OK, (r X \/ s X) => backchain for q X gives two solutions
+Is it important that the substitution in the Or note, X is a function?
+*)
+
+Set Implicit Arguments.
+Inductive typecheck A :=
+  | ty_ok : A -> typecheck
+  | ty_err.
+
+Arguments ty_err {_}.
+
+
 Lemma tm2RC_kp {t1 k} : 
   tm2RC t1 = Some (RCallable_Kp k) -> t1 = Tm_Kp k.
 Proof.
@@ -12,80 +28,25 @@ Qed.
 
 Lemma deref_kp {s1 t k}:
   tm2RC (deref s1 t) = Some (RCallable_Kp k) ->
-    (t = Tm_Kp k) \/ (exists v, t = Tm_V v /\ sigma s1 v = Some (Tm_Kp k)).
+    (t = Tm_Kp k) \/ (exists v, t = Tm_V v /\ lookup v s1 = Some (Tm_Kp k)).
 Proof.
   case: t k => //=.
   - move=> k1 k2 []; left; congruence.
-  - move=> v k; case x: sigma => [t1|]//=.
+  - move=> v k; case x: lookup => [t1|]//=.
     move=>/tm2RC_kp?; subst.
     right; by eexists.
   - move=> h b k; case X: tm2RC => //.
 Qed.
 
-Section checker.
-  Definition sigV := V -> option S.
-
-  Fixpoint is_det_sig (sig:S) : bool :=
-    match sig with
-    | b (d Func) => true
-    | b (d Pred) => false
-    | b Exp => false
-    | arr _ _ s => is_det_sig s
-    end.
-
-  Fixpoint getS_Callable (sP: sigT) (t: Callable) : option S :=
-    match t with
-    | Callable_Kp pn => Some (sP pn)
-    | Callable_V vn => None (*TODO: use sV vn instead*)
-    | Callable_Comb hd _ => getS_Callable sP hd
-    end.
-
-  Fixpoint rcallable_is_det (sP: sigT) (t:RCallable) : bool :=
-    match t with
-    | RCallable_Comb h _ => rcallable_is_det sP h
-    | RCallable_Kp k => is_det_sig (sP k)
-    end.
-
-  Definition tm_is_det (sP: sigT) (t : Callable) :=
-    odflt false (omap is_det_sig (getS_Callable sP t)).
-
-  Definition check_atom sP (a: A) :=
-    match a with
-    | ACut => true
-    | ACall t => tm_is_det sP t
-    end. 
-
-  Fixpoint check_atoms (sP :sigT) (s: seq A) :=
-    match s with
-    | [::] => false
-    | ACut :: xs => all (check_atom sP) xs || check_atoms sP xs
-    | ACall _ :: xs => check_atoms sP xs
-    end.
-
-
-  Definition check_rule sP head prems :=
-    (rcallable_is_det sP head == false) || 
-      check_atoms sP prems.
-
-  Definition check_rules sP rules :=
-    all (fun x => check_rule sP x.(head) x.(premises)) rules.
-
-  Definition check_program sP := 
-    forall pr, check_rules sP (rules pr).
-End checker.
-
-Section check.
-
+Section has_cut.
+  (* tells if A has a superficial cut *)
   Fixpoint has_cut A :=
     match A with
-    | CutS => true
-    | CallS _ _ => false
-    | Bot | Dead => true
-    | OK => false
+    | CutS | Bot | Dead => true
+    | OK | CallS _ _ => false
     | And A B0 B => has_cut A || (has_cut B0 && has_cut B)
     | Or _ _ _ => is_ko A
     end.
-
 
   Lemma has_cut_cut {B}: has_cut (cutr B).
   Proof. 
@@ -94,159 +55,22 @@ Section check.
     - by move=> A ->.
   Qed.
 
-  Lemma has_cut_dead {A}: is_dead A -> has_cut A.
-  Proof.
-    elim: A => //=.
-    - move=> A HA s B HB/andP[/is_dead_is_ko->/is_dead_is_ko->]//.
-    - move=> A HA B0 _ B HB dA; rewrite HA//.
-  Qed.
+  Lemma is_ko_has_cut {A}: is_ko A -> has_cut A.
+  Proof. elim: A => //=; move=> A HA B0 _ B HB dA; rewrite HA//. Qed.
 
-  (* a tree is deterministic if it call deterministic atoms. 
-    delicate cases are And and Or subtrees.
-
-    "((A, !, A') ; B) , C" is OK due to the cut in LHS of Or
-    "((A, A') ; B) , !, C" is OK because any alt from first conjunct dies
-    "((A, A') ; B) , C" is OK if B is dead already (cutr by predecessor of A for example)
-  
-  *)
-  Fixpoint det_tree (sP:sigT) A :=
-    match A with
-    | CutS => true
-    | CallS _ a => tm_is_det sP a
-    | Bot | OK => true
-    | Dead => true
-    | And A B0 B =>
-      (is_ko A) || 
-        [&& (has_cut B0 && has_cut B) || det_tree sP A, 
-          det_tree sP B & det_tree sP B0]
-    | Or A _ B =>
-        det_tree sP A && 
-          if has_cut A then det_tree sP B else (B == cutr B)
-    end.
-
-  Lemma no_alt_cut {sP A}: det_tree sP (cutr A).
-  Proof.
-    elim: A => //.
-    + by move=> A HA s B HB /=; rewrite HA HB cutr2 eqxx if_same.
-    + move=> A HA B0 HB0 B HB /=; rewrite is_ko_cutr//.
-  Qed.
-
-  Lemma no_alt_dead {sP A}: is_dead A -> det_tree sP A.
-  Proof.
-    elim: A => //.
-    + move=> A HA s B HB /=/andP[dA]; rewrite HA// has_cut_dead//.
-    + move=> A HA B0 HB0 B HB /=dA; rewrite is_dead_is_ko//.
-  Qed.
+  Lemma is_dead_has_cut {A}: is_dead A -> has_cut A.
+  Proof. move=> /is_dead_is_ko /is_ko_has_cut//. Qed.
 
   Lemma has_cut_cutl {A}: has_cut A -> has_cut (cutl A).
   Proof.
     elim: A => //.
       move=> A HA s B HB/=/andP[kA kB]; rewrite fun_if/= is_ko_cutr kA !is_ko_cutl// if_same//.
-    move=> A HA B0 HB0 B HB /=; rewrite fun_if/=.
-    rewrite !has_cut_cut/=.
-    case:ifP => // _.
-    move=> /orP[].
-      by move=>/HA->.
-    move=>/andP[cB0] /HB->; rewrite orbT//.
+    move=> A HA B0 HB0 B HB /=/orP[cA|/andP[cB0 cB]].
+      by rewrite fun_if/=HA//= has_cut_cut if_same.
+    by rewrite fun_if /= HB// !has_cut_cut orbT if_same.
   Qed.
 
-  Lemma all_det_nfa_big_and {p sP l}: all (check_atom sP) l -> det_tree sP (big_and p l).
-  Proof.
-    elim: l => //= a l IH/andP[] H1 H2.
-    case: a IH H1 => //= [|t] IH H1; rewrite ?H1 IH//=orbT//.
-  Qed.
-
-  Lemma cut_followed_by_det_has_cut {sP p l}:
-      check_atoms sP l -> has_cut (big_and p l).
-  Proof. by elim: l => //= -[]//= _ l H/H->. Qed.
-
-  Lemma cut_followed_by_det_nfa_and {sP p bo} :
-    check_atoms sP bo -> det_tree sP (big_and p bo).
-  Proof.
-    elim: bo => //=.
-    move=> [|t] /= l IH.
-      by move=>/orP[/all_det_nfa_big_and|/IH]->; rewrite orbT.
-    by move=> H; rewrite IH//!andbT andbb (cut_followed_by_det_has_cut H).
-  Qed.
-
-  Lemma no_free_alt_cutl {sP A}: det_tree sP (cutl A).
-  Proof.
-    elim: A => //.
-      move=> A HA s B HB/=.
-      rewrite fun_if/=HA HB cutr2 eqxx no_alt_cut if_same.
-      case: ifP => //dA.
-      rewrite has_cut_dead//no_alt_dead//.
-    move=> A HA B0 HB0 B HB /=.
-    rewrite fun_if/= HA HB !has_cut_cut/= !no_alt_cut/= !orbT if_same//.
-  Qed.
-
-  Variable u : Unif.
-
-  Lemma tiki_taka {sP s s3 modes t q hd1}:
-    let t' := tm2RC (deref s (Callable2Tm t)) in
-    t' = Some q ->
-    tm_is_det sP t ->
-      H u modes q hd1 s = Some s3 ->
-        rcallable_is_det sP hd1.
-  Proof.
-    move=>/=.
-    elim: modes q hd1 t s s3 => //=.
-      move=> []//=k []//= k1 t s1 s2; case: eqP => //=<-.
-      move=>/deref_kp [].
-        case: t => //= k2 [->]//.
-      move=> [v[]]; case: t => //.
-    move=> []//ml IH []//h1 b1 []//=h2 b2 t s1 s2 H1 H2 H3.
-      move: H3; case e: H => //=[s1'] H3.
-      case: t H1 H2 => //= c t.
-      case H : tm2RC => //=[h1'] [??]; subst => /=.
-      rewrite/tm_is_det/=.
-      case X: getS_Callable => //[S] H1.
-      apply: IH H _ e.
-      rewrite/tm_is_det X//.
-    move: H3; case e: H => //=[s1'] H3.
-    case: t H1 H2 => //= c t.
-    case H : tm2RC => //=[h1'] [??]; subst => /=.
-    rewrite/tm_is_det/=.
-    case X: getS_Callable => //[S] H1.
-    apply: IH H _ e.
-    rewrite/tm_is_det X//.
-  Qed.
-
-
-  Lemma is_det_no_free_alt {sP t s1} {p:program}:
-    check_rules sP p.(rules) -> tm_is_det sP t -> 
-      det_tree sP (big_or u p s1 t).
-  Proof.
-    rewrite /big_or/F.
-    case X: tm2RC => //=[q].
-    case: p => rules modes sig1 /=.
-    generalize {| rules := rules; modes := modes; sig := sig1 |} as pr => pr.
-    clear -X.
-    elim: rules modes s1 t pr q X => //=.
-    move=> [] hd bo rules IH modes s/= t p q X /andP[H1 H1'] H2.
-    case H: H => /= [s2|]; last first.
-      apply: IH X H1' H2.
-    clear IH.
-    move: H.
-    move: H1 => /orP[]; last first.
-      move=> + _.
-      elim: rules H1' bo => //=.
-        move=> _ bo.
-        apply cut_followed_by_det_nfa_and.
-      move=> [] hd1 bo1/= l IH /andP [H3 H4] bo H1.
-      case H: H => [s3|]//=; last first.
-        by apply: IH.
-      rewrite (cut_followed_by_det_has_cut H1).
-      rewrite cut_followed_by_det_nfa_and//=.
-      rewrite IH//=.
-      move: H3 => /orP[] => //.
-      move=> /eqP H3; exfalso.
-      have /= := tiki_taka X H2 H; congruence.
-    move=> /eqP H3 H4.
-    have /= := tiki_taka X H2 H4; congruence.
-  Qed.
-
-  Lemma expand_has_cut {A s}: 
+  Lemma expand_has_cut {u A s}: 
     has_cut A -> has_cut (get_tree (expand u s A)) \/ is_cutbrothers (expand u s A).
   Proof.
     elim: A s; try by move=> /=; auto.
@@ -262,54 +86,9 @@ Section check.
         by case: ifP; rewrite ?cC // has_cut_cutl.
       case/andP=> cB0 cB.
       case: expand => [|||] C/=; rewrite ?cB ?cB0 ?orbT; auto.
-      move: (HB (get_substS s C)).
+      move: (HB (get_substS s C) cB).
       by case: expand => [|||] D /=; auto => -[]// ->; rewrite cB0 orbT; left.
   Qed.
-
-  Lemma expand_no_free_alt {sP s1 A r} : 
-    check_program sP -> det_tree sP A -> 
-      expand u s1 A = r ->
-        det_tree sP (get_tree r).
-  Proof.
-    move=> H + <-; clear r.
-    elim: A s1 => //.
-    - move=> p t s1 /=.
-      apply: is_det_no_free_alt.
-      by have:= H p.
-    - move=> A HA s B HB s1 /=/andP[fA].
-      case: ifP => //= cA.
-        move=> nnB.
-        case: ifP => //= dA.
-          have:= HB s1 nnB.
-          case: expand => //= [|||] C nnC/=; rewrite get_tree_Or/=fA/=cA?HB//.
-        have:= HA s1 fA.
-        have := @expand_has_cut _ s1 cA.
-        case X: expand => //= -[]// + ->; rewrite ?nnB ?no_alt_cut //=; try by case: has_cut.
-        by rewrite cutr2 eqxx if_same.
-      move/eqP->.
-      case: ifP => [dA|].
-        rewrite get_tree_Or/=cA no_alt_dead//=is_ko_expand//=?is_ko_cutr//cutr2//.
-      have:= HA s1 fA => + dA.
-      case Y: expand => /=->; rewrite !cutr2 eqxx no_alt_cut if_same//.
-    - move=> A HA B0 HB0 B HB s /=.
-      move=>/orP[].
-        move=>kA; rewrite is_ko_expand///=kA//.
-      move=> /and3P[/orP[/andP[cB0 cB]|fA] fB fB0].
-        case X: expand => //= [|||C]; try rewrite cB0 cB/= fB0 fB !orbT//.
-        rewrite get_tree_And.
-        rewrite /= (HB (get_substS s C)) //.
-        have := @expand_has_cut _ (get_substS s C) cB.
-        case H1: (is_cutbrothers (expand u (get_substS s C) B)).
-          move=>_/=; rewrite has_cut_cut// no_free_alt_cutl no_alt_cut !orbT//.
-        move=> []//H2; rewrite H2 fB0 cB0 orbT//.
-      have:= HA s fA.
-      case X: expand => //= [|||C] H1; try rewrite H1 orbT fB fB0 orbT//.
-      have:= HB (get_substS s C) fB; case Y: expand => //= H2; try rewrite fB0 H2 H1 orbT !orbT//.
-      rewrite !no_free_alt_cutl no_alt_cut H2 !orbT//.
-  Qed.
-
-  Goal forall sP s, det_tree sP (Or OK s OK) == false.
-  Proof. move=> ?? //=. Qed.
 
   Lemma has_cut_success {A}:
     has_cut A -> success A = false.
@@ -331,33 +110,6 @@ Section check.
       move=>/success_is_ko->//.
     - by move=> A HA B0 HB0 B HB/=/andP[]/HA->/HB->; rewrite andbF.
   Qed.
-
-  Lemma expand_next_alt {sP A} : 
-    check_program sP -> det_tree sP A -> success A ->
-      next_alt true A = None.
-  Proof.
-    move=> H; elim: A => //=.
-    - move=> A HA s B HB /andP[nA IH].
-      case: ifP => [dA sB|dA sA].
-        rewrite is_dead_next_alt// HB//.
-        move: IH; case: ifP => //.
-        move=> _ /eqP->; rewrite no_alt_cut//.
-      rewrite HA//.
-      move: IH; case: ifP.
-        move=> /has_cut_success; congruence.
-      move=> _ /eqP->; rewrite next_alt_cutr//.
-    - move=> A HA B0 HB0 B HB /orPT[].
-        move=> /is_ko_success->//.
-      move=> /and3P[/orP[/andP[cB0 cB]|fA] fB fB0]/andP[sA sB].
-        rewrite success_has_cut// in cB.
-      rewrite success_failed//sA.
-      rewrite HB//HA//.
-  Qed.
-
-  Lemma build_na_is_dead {sP A}:
-    check_program sP -> det_tree sP A -> success A ->
-      (build_na A (next_alt true A)) = dead A.
-  Proof. move=> H1 H2 H3; by rewrite (expand_next_alt H1)//=. Qed.
 
   Lemma has_cut_next_alt {A B b}: 
     has_cut A -> next_alt b A = Some B -> has_cut B.
@@ -401,150 +153,847 @@ Section check.
         by rewrite cB0 (HB0 _ _ cB0 Z) orbT.
       by move=> [<-]/=; rewrite cB0 cB orbT.
   Qed.
+End has_cut.
 
-  Lemma no_free_alt_next_alt {sP A B b}:
-    det_tree sP A -> next_alt b A = Some B -> det_tree sP B.
-  Proof.
-    elim: A B b => //=.
-    - move=> /= B b _; case: ifP => // _[<-]//.
-    - move=> p c B _ _ [<-]//.
-    - move=> B _ _ [<-]//.
-    - move=> A HA s B HB C /= b.
-      move=>/andP[fA].
-      case: (ifP (is_dead _)) => dA.
-        rewrite is_dead_next_alt//.
-        rewrite has_cut_dead//.
-        move=> fB.
-        have:= HB _ b fB.
-        case X: next_alt => //[D] /(_ _ erefl) fD[<-]/=.
-        rewrite no_alt_dead//?is_dead_dead//has_cut_dead// is_dead_dead//.
-      case: ifP => cA.
-        move=> fB.
-        have:= (HA _ b fA).
-        case X: next_alt => //[D|].
-          have cD:= has_cut_next_alt cA X.
-          by move=> /(_ _ erefl) fD[<-]/=; rewrite fD cD fB.
-        move=> _.
-        have idA := @is_dead_dead A.
-          case Y: next_alt => //[D].
-          move=>[<-]/=.
-          rewrite no_alt_dead// has_cut_dead//.
-          apply: HB fB Y.
-      move=>/eqP->; rewrite (is_ko_next_alt _ is_ko_cutr).
-      have:= HA _ b fA.
-      case: next_alt; rewrite ?if_same// => D /(_ _ erefl) fD [<-]/=.
-      by rewrite fD cutr2 eqxx no_alt_cut if_same.
-    - move=> A HA B0 HB0 B HB C b /=.
-      move=>/orP[].
-        move=>kA.
-        by rewrite is_ko_failed// is_ko_next_alt//.
-      move=> /and3P[/orP[/andP[cB0 cB]|fA] fB fB0].
-        case: ifP => // fA.
-          case X: next_alt => // [A'].
-          case Y: next_alt => //[B0'] [<-]/=.
-          by rewrite cB0 fB0 (has_cut_next_alt cB0 Y) (HB0 _ _ fB0 Y) orbT.
-        case: ifP => sA; last first.
-          by move=> [<-]/=; rewrite cB0 cB fB fB0 orbT.
-        have:= HB _ b fB.
-        case X: next_alt => // [B'|].
-          by move=> /(_ _ erefl) fD [<-]/=; rewrite cB0  (has_cut_next_alt cB X) (HB _ _ fB X) fB0 orbT.
-        move=> _; case Y: next_alt => //[A'].
-        by case Z: next_alt => //[B0'][<-]/=; rewrite cB0 (has_cut_next_alt cB0 Z) (HB0 _ _ fB0 Z) fB0 orbT.
-      case: ifP => // _.
-        case X: next_alt => // [A'].
-        case Y: next_alt => // [B0'][<-]/=.
-        by rewrite (HA _ _ fA X) fB0 (HB0 _ _ fB0 Y) !orbT.
-      case: ifP => sA; last first.
-        by move=>[<-]/=; rewrite fA fB fB0 !orbT.
-      case X: next_alt => // [B'|].
-        by move=> [<-]/=; rewrite fA fB0 (HB _ _ fB X)!orbT.
-      case Y: next_alt => // [A'].
-      case Z: next_alt => //[B0'] [<-]/=.
-      by rewrite (HA _ _ fA Y) (HB0 _ _ fB0 Z) fB0 !orbT.
-  Qed.
+Definition full_sP {K:eqType} {V:Type} (s: list (K*V)) := forall k, lookup k s <> None.
+Notation sigV := (list (V * S)).
 
-  Lemma expand_next_alt_failed {sP A B C s b}:
-    check_program sP ->
-      det_tree sP A -> expand u s A = Failure B ->
-        next_alt b B = Some (C) -> det_tree sP C.
-  Proof.
-    move=> H1 H2 H3 H4.
-    have /= H5 := expand_no_free_alt H1 H2 H3.
-    by have:= no_free_alt_next_alt H5 H4.
-  Qed.
+Section checker.
 
-  Lemma no_free_alt_dead {sP A}:
-    is_dead A -> det_tree sP A.
-  Proof.
-    elim: A => //=.
-    - move=> A HA s B HB /andP[dA dB]; by rewrite has_cut_dead//HA//HB.
-    - by move=> A HA B0 _ B HB dA; rewrite is_dead_is_ko//.
-  Qed.
+  Fixpoint is_det_sig (sig:S) : bool :=
+    match sig with
+    | b (d Func) => true
+    | b (d Pred) => false
+    | b Exp => false
+    | arr _ _ s => is_det_sig s
+    end.
 
-  Definition is_det A := forall b s s' B,
-    runb u s A s' B b -> is_dead B.
+  Fixpoint get_tm_hd_sig (sP : sigT) (sV : sigV) (tm: Tm) : option S :=
+    match tm with
+    | Tm_Kd _ => (Some (b Exp))
+    | Tm_Kp k => (lookup k sP) (*TODO: sP should be complete*)
+    | Tm_V v => lookup v sV
+    | Tm_Comb h _ => get_tm_hd_sig sP sV h
+    end.
 
-  Lemma runb_next_alt {sP A}: 
-    check_program sP -> 
-      det_tree sP A -> is_det A.
-  Proof.
-    rewrite/is_det.
-    move=> H1 H2 b s s' B H3.
-    elim: H3 H2; clear -H1 => //.
-    - move=> s1 s2 A B sA _ <- fA.
-      by rewrite (build_na_is_dead H1 fA sA) is_dead_dead.
-    - move=> s1 s2 r A B n eA rB IH fA.
-      by apply: IH; apply: expand_no_free_alt eA.
-    - move=> s1 s2 r A B n eA rB IH fA.
-      by apply: IH; apply: expand_no_free_alt eA.
-    - move=> s1 s2 A B r n fA nA H IH FA.
-      apply: IH.
-      apply: no_free_alt_next_alt FA nA.
-    - by move=> *; rewrite is_dead_dead.
-  Qed.
+  Definition get_callable_hd_sig (sP: sigT) sV (t: Callable) : option S :=
+    get_tm_hd_sig sP sV (Callable2Tm t).
 
-  Lemma main {sP p t}:
-    check_program sP -> tm_is_det sP t -> 
-      is_det ((CallS p t)).
-  Proof.
-    move=> H1 fA HA.
-    apply: runb_next_alt H1 _ HA.
-    apply: fA.
-  Qed.
+  Definition callable_is_det (sP: sigT) sV (t : Callable) :=
+    odflt false (omap is_det_sig (get_callable_hd_sig sP sV t)).
 
-  Print Assumptions  main.
+  Definition maxD (d1 d2 : D) :=
+    match d1, d2 with
+    | Pred, _ | _, Pred => Pred
+    | Func, Func => Func
+    end.
+
+  Definition minD (d1 d2 : D) :=
+    match d1, d2 with
+    | Func, _ | _, Func => Func
+    | Pred, Pred => Pred
+    end.
+
+  Lemma maxD_refl {r}: maxD r r = r.
+  Proof. case: r => //. Qed.
+
+  Lemma maxD_comm {l r}: maxD l r = maxD r l.
+  Proof. case: l; case: r => //. Qed.
+
+  Lemma minD_refl {r}: minD r r = r.
+  Proof. case: r => //. Qed.
+
+  Lemma minD_comm {l r}: minD l r = minD r l.
+  Proof. case: l; case: r => //. Qed.
+
+  Lemma maxD_assoc {x y z}: maxD x (maxD y z) = maxD (maxD x y) z.
+  Proof. case: x => //=; case: y => //=; case: z => //. Qed.
+
+  Lemma minD_assoc {x y z}: minD x (minD y z) = minD (minD x y) z.
+  Proof. case: x => //=; case: y => //=; case: z => //. Qed.
+
+  Definition map_ty {A B} (F: A -> typecheck B) (ob1: typecheck A) : (typecheck B) :=
+    match ob1 with
+    | ty_err => ty_err
+    | ty_ok cnt => F cnt
+    end.
+
+  Definition map_ty_bool ob1 ob2 : typecheck bool :=
+    map_ty (fun x => map_ty (fun y => ty_ok (x && y)) ob1)  ob2.
+
+  Fixpoint incl_aux f1 f2 s1 s2 : typecheck _:=
+    match s1, s2 with
+    | b Exp, b Exp => ty_ok true
+    | b(d D1), b(d D2) => ty_ok (f1 D1 D2 == D1)
+    | arr i l1 r1, arr i l2 r2 => map_ty_bool (incl_aux f2 f1 l1 l2) (incl_aux f1 f2 r1 r2)
+    | arr o l1 r1, arr o l2 r2 => map_ty_bool (incl_aux f1 f2 l1 l2) (incl_aux f1 f2 r1 r2)
+    | _, _ => ty_err
+    end.
+
+  Definition map_ty_s m (ob1:typecheck S) ob2 : typecheck S :=
+    map_ty (fun x => map_ty (fun y => ty_ok (arr m x y)) ob2) ob1.
+
+  Fixpoint min_max f1 f2 s1 s2 : typecheck _ :=
+    match s1, s2 with
+    | b Exp, b Exp => ty_ok (b Exp)
+    | b(d D1), b(d D2) => ty_ok (b(d(f1 D1 D2)))
+    | arr i l1 r1, arr i l2 r2 => map_ty_s i (min_max f2 f1 l1 r1) (min_max f1 f2 r1 r2)
+    | arr o l1 r1, arr o l2 r2 => map_ty_s o (min_max f1 f2 l1 r1) (min_max f1 f2 r1 r2)
+    | _, _ => ty_err
+    end.
+
+  Definition incl := incl_aux minD maxD.
+  Definition min := min_max minD maxD.
   
-  Section tail_cut.
+  Fixpoint strong s :=
+    match s with
+    | b Exp => b Exp
+    | b(d _) => b(d Func)
+    | arr i l r => arr i (weak l) (strong r)
+    | arr o l r => arr o (strong l) (strong r)
+    end
+  with weak s :=
+    match s with
+    | b Exp => b Exp
+    | b(d _) => b(d Pred) 
+    | arr i l r => arr i (strong l) (weak r)
+    | arr o l r => arr o (weak l) (weak r)
+    end.
 
-    Definition tail_cut (r : R) :=
-    match r.(premises) with [::] => false | x :: xs => last x xs == ACut end.
-    
-    Definition AllTailCut := (forall pr : program, all tail_cut (rules pr)).
+  Section test.
+    Definition SMap := 
+      (arr i (arr i (b Exp) (arr o (b Exp) (b(d Func)))) (arr i (b Exp) (arr o (b Exp) (b(d Func))))).
+    Definition WMap := 
+      (arr i (arr i (b Exp) (arr o (b Exp) (b(d Func)))) (arr i (b Exp) (arr o (b Exp) (b(d Pred))))).
+    Goal incl SMap WMap = ty_ok true. Proof. move=>//=. Qed.
+    Goal  (incl WMap SMap) = ty_ok false. Proof. move=>//=. Qed.
+    Goal (weak SMap) == WMap. Proof. move=> //=. Qed.
+  End test.
 
-    Lemma cut_in_prem_tail_cut sP: AllTailCut -> check_program sP.
-    Proof.
-      rewrite /AllTailCut /check_program.
-      rewrite /tail_cut /check_rules.
-      move=> + pr => /(_ pr).
-      remember (rules pr) as RS.
-      apply: sub_all => r; clear.
-      rewrite /check_rule.
-      case X: rcallable_is_det => //=.
-      case: r X => //= hd []//= + l.
-      elim: l => //=.
-      move=> x xs IH []//=; last first.
-        move=> _; apply IH.
-      by move=> H1 H2; rewrite IH//orbT.
-    Qed.
+  Definition map_ty_opt {A B: Type} (f: A -> typecheck (option B)) t :=
+    match t with
+    | ty_ok (Some e) => (f e)
+    | ty_err => ty_err
+    | ty_ok None => ty_ok (@None B)
+    end.
 
-    Lemma tail_cut_is_det sP p t:
-      AllTailCut -> tm_is_det sP t -> is_det ((CallS p t)).
-    Proof.
-      move=> /(cut_in_prem_tail_cut sP).
-      apply main.
-    Qed.
-  End tail_cut.
+  (* takes a tm and returns its signature + if it is well-called
+     the tm has no signature if its head is a variable with no assignment in sV *)
+  Fixpoint check_tm (sP:sigT) (sV:sigV) (tm : Tm) : typecheck (option (S * bool)) :=
+    match tm with
+    | Tm_Kd k => ty_ok (Some (b Exp, true))
+    | Tm_Kp k => ty_ok (omap (fun x => (x, true)) (lookup k sP)) (*TODO: sP should be complete*)
+    | Tm_V v => ty_ok (omap (fun x => (x, true)) (lookup v sV))
+    | Tm_Comb l r => 
+      map_ty_opt (
+        fun '(s1, b1) => 
+        match s1 with
+          | arr i tl tr => 
+            map_ty_opt (fun '(s2, b2) =>
+              map_ty (fun bi => 
+                ty_ok (Some (if b1 && b2 && bi then (tr, true) else (weak tr, false)))
+              ) (incl s2 tl))
+            (check_tm sP sV r)
+          | arr o tl tr => if b1 then (check_tm sP sV l) else ty_ok (Some (weak tr, false))
+          | _ => ty_err
+          end
+      ) (check_tm sP sV l)
+    end.
 
-  Print Assumptions tail_cut_is_det.
+  (* takes a tm and a signature and updates variable signatures
+     updates are performed only on toplevel variables or variables in input positions *)
+  Fixpoint assume_tm (sP:sigT) (sV:sigV) (tm : Tm) (s : S): typecheck sigV :=
+    match tm with
+    | Tm_Kd _ | Tm_Kp _ => ty_ok sV (*TODO: should I raise ty_err if mismatch between s and type(tm)? *)
+    | Tm_V v =>
+      if lookup v sV is Some s' then map_ty (fun s'' => ty_ok (add v s'' sV)) (min s s')
+      else ty_ok (add v s sV)
+    | Tm_Comb l r =>
+      match s with
+      | arr i tl tr =>
+        map_ty (fun sP' => assume_tm sP sP' r tr) (assume_tm sP sV l tl)
+      | arr o tl tr => assume_tm sP sV l tl
+      | _ => ty_err
+      end
+    end.
+
+  (* assumes the output tm and then it goes on inputs *)
+  Fixpoint assume_call (sP:sigT) (sV:sigV) (c : Callable) (s : S): typecheck sigV :=
+    match c with
+    | Callable_Kp _ => ty_ok sV (*TODO: should I raise ty_err if mismatch between s and type(c)? *)
+    | Callable_V v => ty_ok sV
+    | Callable_Comb l r =>
+      match s with
+      | arr i tl tr => assume_call sP sV l tl
+      | arr o tl tr => 
+        map_ty (fun sV' => assume_tm sP sV' r tr) (assume_call sP sV l tl)
+      | _ => ty_err
+      end
+    end.
+
+  (* assumes variables in input positions *)
+  Fixpoint assume_hd (sP:sigT) (sV:sigV) (s : S) (tm:Tm) : typecheck sigV :=
+    match tm with
+    | Tm_Kd _ => ty_ok sV
+    | Tm_Kp _ => ty_ok sV
+    | Tm_V v =>
+      if lookup v sV is Some s' then
+        map_ty (fun s'' => ty_ok (add v s'' sV)) (min s s')
+      else 
+        ty_ok (add v s sV)
+    | Tm_Comb l r => 
+      match s with
+      | arr i tl tr => 
+        map_ty (fun sV' => assume_hd sP sV' tr r) (assume_hd sP sV tl l)
+      | arr o tl _ => (assume_hd sP sV tl l)
+      | _ => ty_err
+      end
+    end.
+
+  (* verifies variables in outputs positions *)
+  Fixpoint check_hd (sP:sigT) (sV:sigV) (s : S) (tm:Tm) : typecheck bool :=
+    match tm with
+    | Tm_Kd _ => incl (b Exp) s
+    | Tm_Kp k => odflt (ty_ok false) (omap (fun x => incl x s) (lookup k sP)) (*TODO: sP should be complete*)
+    | Tm_V v => 
+      if lookup v sV is Some s' then incl s' s
+      else ty_ok false
+    | Tm_Comb l r => 
+      match s with
+      | arr i tl _ => (check_hd sP sV tl l)
+      | arr o tl tr => 
+        match  (check_tm sP sV r) with
+        | ty_err => ty_err
+        | ty_ok None => ty_ok false
+        | ty_ok (Some (t, b1)) => 
+          map_ty 
+            (fun b2 => map_ty (fun bi => ty_ok (bi && b1 && b2)) (incl t s))
+          (check_hd sP sV tl l) 
+        end 
+      | _ => ty_err
+      end
+    end.
+
+  (* checks inputs and assumes outputs of a callable *)
+  Definition check_callable sP sV (c: Callable) d : typecheck (D * sigV) :=
+    match check_tm sP sV (Callable2Tm c)  with
+    | ty_err => ty_err
+    | ty_ok None => ty_ok (Pred, sV)
+    | ty_ok (Some ((b Exp | arr _ _ _), _)) => ty_err (*NOTE: callable have type prop!*)
+    | ty_ok (Some ((b(d x)), b1)) =>
+      if b1 then 
+        if get_callable_hd_sig sP sV c is Some s then
+          map_ty (fun sV' => ty_ok (maxD x d, sV')) (assume_call sP sV c s)
+        else ty_ok (Pred, sV)
+      else ty_ok (Pred, sV)
+    end.
+
+  Definition check_atom sP sV (a: A) (s:D) : typecheck (D * sigV) :=
+    match a with
+    | ACut => ty_ok (Func, sV)
+    | ACall t => check_callable sP sV t s
+    end. 
+
+  (* takes a list of atoms and returns if they typecheck, their determinacy, the updated sigV *)
+  Fixpoint check_atoms sP sV l s :=
+    match l with
+    | [::] => ty_ok (s, sV)
+    | x :: xs => 
+      map_ty (fun '(s', sV') => check_atoms sP sV' xs s') (check_atom sP sV x s)
+    end.
+
+  Fixpoint RCallable2Callable rc := 
+    match rc with
+    | RCallable_Comb h bo => Callable_Comb (RCallable2Callable h) bo
+    | RCallable_Kp k => Callable_Kp (k)
+    end.
+
+  Fixpoint RCallable_sig (sP: sigT) (t:RCallable) :=
+    match t with
+    | RCallable_Comb h _ => RCallable_sig sP h
+    | RCallable_Kp k => (lookup k sP) (*TODO: sP should be complete*)
+    end.
+
+  Definition empty_ctx : sigV := [::].
+  
+  (* The rules passes the check if:
+     - it is implementing a function or a relation, the body is function, the outputs are ok
+  *)
+  Definition check_rule sP sV head prems :=
+    let hd_sig := RCallable_sig sP head in
+    match hd_sig with
+    | None => ty_err
+    | Some hd_sig => 
+        (let is_det_head := is_det_sig hd_sig in
+        let tm_head := (Callable2Tm (RCallable2Callable head)) in
+        let ass_hd := assume_hd sP sV hd_sig tm_head in
+        map_ty (fun '(sV') => 
+          let ck_A := check_atoms sP sV' prems Func in
+          map_ty (fun '(b1, sV'') =>
+            if is_det_head && (b1 == Pred) then ty_ok false
+            else check_hd sP sV'' hd_sig tm_head) ck_A) ass_hd)
+    end.
+
+  Definition check_rules sP sV rules :=
+    all (fun x => 
+      match check_rule sP sV x.(head) x.(premises) with 
+      | ty_ok b1 => b1 
+      | ty_err => false
+      end) rules.
+
+  Definition check_program sP := 
+    forall pr, check_rules sP empty_ctx (rules pr).
+End checker.
+
+(* a free alternative can be reached without encountering a cutr following SLD 
+
+  "((A, !, A') ; B) , C" is OK since B is not free
+  "((A, A') ; B) , !, C" is OK because any alt from first conjunct dies
+  "((A, A') ; B) , C" is OK if B is dead already (cutr by predecessor of A for example)
+
+*)
+Fixpoint det_tree_aux (sP:sigT) (sV : sigV) A dd : typecheck (D * sigV) :=
+  match A with
+  | CutS => ty_ok (Func, sV)
+  | CallS _ a => 
+    map_ty (fun '(dd', sV') =>  ty_ok (maxD dd dd', sV')) (check_callable sP sV a dd)
+  | Bot | OK | Dead => ty_ok (dd, sV)
+  | And A B0 B =>
+    if is_ko A then ty_ok (dd, sV)
+    else
+      let rA := (det_tree_aux sP sV A dd) in
+      map_ty (fun '(dd', sV') =>
+        let rB0 := (det_tree_aux sP sV' B0 dd') in
+        let rB := (det_tree_aux sP sV' B dd') in
+        map_ty (fun '(ddB0, sVB0) =>
+          map_ty (fun '(ddB, sVB) =>
+            ty_ok (maxD ddB0 ddB, sV')) rB) rB0) rA
+  | Or A _ B =>
+      (* TODO: should use the substitution s before running the check on B?
+         if so, it is no needed to verify that the state is valid
+      *)
+      map_ty (
+        fun '(sVA, sV') => 
+        map_ty (fun '(sVB, _) =>
+      if has_cut A then ty_ok (maxD sVA sVB, sV) else 
+      if (is_ko B) then ty_ok (sVA, sV')
+      else ty_ok (Pred, sV)) (det_tree_aux sP sV B dd)) (det_tree_aux sP sV A dd)
+  end.
+
+Definition typ_func (A: typecheck (_ * sigV)) := match A with ty_ok (Func, _) => true | _ => false end.
+
+Definition det_tree sP A := typ_func (det_tree_aux sP empty_ctx A Func).
+
+Lemma no_alt_ko {sP A}: is_ko A -> det_tree sP A.
+Proof.
+  rewrite/det_tree.
+  elim: A => //.
+  + move=> A HA s B HB /=/andP[kA kB].
+    case X: det_tree_aux HA => //=[[[] sVA]|]/(_ kA)//.
+    case Y: det_tree_aux HB => //=[[[] sVB]|]/(_ kB)//=.
+    rewrite is_ko_has_cut//.
+  + move=> A HA B0 HB0 B HB /= ->//.
+Qed.
+
+Lemma no_alt_cut {sP A}: det_tree sP (cutr A).
+Proof. apply: no_alt_ko is_ko_cutr. Qed.
+
+
+Lemma no_alt_dead {sP A}: is_dead A -> det_tree sP A.
+Proof. move=>/is_dead_is_ko. apply: no_alt_ko. Qed.
+
+Lemma all_det_nfa_big_and {sP sV l r} p: 
+  typ_func (check_atoms sP sV l r)-> 
+    typ_func (det_tree_aux sP sV (big_and p l) r).
+Proof.
+  elim: l sV r => //=.
+  move=> A As IH sV r.
+  case X: check_atom => [[dA sVA]|]//=.
+  case YY : A X => //=[|c].
+    move=> [??]; subst => //=.
+    move=> {}/IH H.
+    case: det_tree_aux H => //=-[]//[]//.
+  rewrite/check_callable.
+  case X: check_tm => //[[[d b]|]]//=; last first.
+    move=> [??]; subst => /=; rewrite maxD_comm/=.
+    move=> /IH/=; case: det_tree_aux => //-[]/=[]//.
+  case: d X => //-[]//=d.
+  case Y: get_callable_hd_sig => //[s|].
+    case: b => //=.
+      case X: assume_call => //=[ts] H [??]; subst.
+      move=> /IH.
+      rewrite maxD_comm maxD_assoc maxD_refl.
+      case: det_tree_aux => //-[]//=[]//.
+    move=> H [??]; subst => /IH.
+    rewrite maxD_comm/=.
+    case: det_tree_aux => //-[]//=[]//.
+  case: b => //=.
+    move=> H [??]; subst.
+    move=> /IH.
+    rewrite maxD_comm/=.
+    case: det_tree_aux => //-[]//=[]//.
+  move=> H [??]; subst => /IH.
+  rewrite maxD_comm/=.
+  case: det_tree_aux => //-[]//=[]//.
+Qed.
+
+(* Lemma cut_followed_by_det_has_cut {sP sV l} p:
+  check_atoms_w_cut sP sV l -> has_cut (big_and p l).
+Proof. move=>/andP[] _; elim: l => //=-[]//= x xs IH /IH->//. Qed.
+
+Lemma cut_followed_by_det_nfa_and {sP sV bo} p:
+  check_atoms_w_cut sP sV bo -> (det_tree_aux sP sV (big_and p bo) Func).1 = Func.
+Proof. move=>/andP[]/eqP/all_det_nfa_big_and//. Qed. *)
+
+Lemma deterf_empty c: 
+  deref empty c = c.
+Proof. elim: c => //= t IH tm H; rewrite IH//. Qed.
+
+(* Lemma tiki_taka {modes sP u q hd s1 c}:
+  tm2RC (Callable2Tm c) = Some q ->
+  H u (modes q) q hd empty = Some s1 ->
+  check_tm sP empty_ctx (Callable2Tm c) = (b (d Func), true)
+   -> rcallable_is_det sP hd.
+Proof.
+  generalize (modes q) => {}modes/=.
+  elim: modes q hd s1 c => //=.
+    move=> []//=k []//= k1 s1 c; case: eqP => //=?+[?]; subst.
+    elim: c k1 => //=.
+      move=> k k1 [<-][->]//.
+    move=> c IH t k1.
+    case: tm2RC => //.
+  move=> [] ms IH []//= r t []//=r1 tm1 s1 []//=r2 tm2.
+    case X: tm2RC => //=[r3][??]; subst.
+    case Y: H => //=[s3] H1.
+    case Z: check_tm => //=[[|m sx sy]b1]//.
+    case: m Z => H2.
+      case W: check_tm => [sw b2].
+      case: ifP => //; case: b1 H2 => //; case: b2 W => //=.
+      move=> H2 W H3 [?]; subst.
+      admit.
+    admit.
+  case X: tm2RC => //=[r3][??]; subst.
+  case Y: H => //=[s3] H1.
+  case Z: check_tm => //=[[|m sx sy]b1]//.
+  case: m Z => H2.
+    case W: check_tm => [sw b2].
+    case: ifP => //; case: b1 H2 => //; case: b2 W => //=.
+    move=> H2 W H3 [?]; subst.
+    admit.
+  admit.
+Admitted. *)
+
+(* Given a deterministic predicate p,
+  Let t, be a valid call to p,
+  Given a list of valid rules in a program p, then
+  backchaining produces a deterministic tree!
+*)
+
+(* Lemma is_det_det_tree {u} {p c sP}:
+  (forall pr : program, check_rules sP empty_ctx (rules pr)) ->
+  (det_tree_aux sP empty_ctx (CallS p c) Func).1 == Func ->
+  (det_tree_aux sP empty_ctx (big_or u p empty c) Func).1 == Func.
+Proof.
+  rewrite/check_rules/=/check_rule.
+  rewrite/=.
+  rewrite /big_or/F.
+  case X: tm2RC => //[rc].
+  move=> /(_ p).
+  case: p => rules modes sig1 /=.
+  generalize {| rules := rules; modes := modes; sig := sig1 |} as pr => pr.
+  clear -X.
+  rewrite/check_callable.
+  elim: rules modes c pr rc X => //=.
+  move=> [] hd bo rules IH modes /= c p q X /andP[Hx Hy].
+  case Y: check_tm => [s []]//=.
+  case: s Y => // -[]//=d H1.
+  case Z: get_callable_hd_sig => //=[s].
+  rewrite maxD_comm/=.
+  case: d H1 => //= H2 _.
+  have {IH} := IH _ _ _ _ X Hy; rewrite H2/=Z/= => -/(_ modes p erefl).
+  case W: run.H => [s1|]//=.
+  move/orP: Hx => [].
+    rewrite deterf_empty in X.
+    admit. (*TODO: hd = q = c and c is func: *)
+  move=>/[dup]/cut_followed_by_det_nfa_and -/(_ p)+H.
+  case R: select => //=[|x xs].
+    case: det_tree_aux => -[]//.
+  case : x R => [sx bx]/=.
+  case T: det_tree_aux => [dy sr]/=+?; subst => /=.
+  case U: det_tree_aux => //=[[] bw]//=+ _.
+  case: ifP => //=.
+  case: ifP => //=.
+  have:= cut_followed_by_det_has_cut _ H.
+  move=> ->//.
+Admitted. *)
+
+(* INVARIANT: all variables are deref  *)
+Fixpoint sigma2ctx (sP:sigT) (s: Sigma) acc : option sigV :=
+  match s with
+  | [::] => Some (rev acc)
+  | (k,v)::xs => 
+    match check_tm sP empty_ctx v with
+    | ty_err => None
+    | ty_ok (Some (v, b1)) => sigma2ctx sP xs ((k, if b1 then v else weak v)::acc)
+    | ty_ok None => sigma2ctx sP xs acc
+    end
+  end.
+
+(* 
+  Given a checked program, and a deterministic tree,
+  then calling expand produces a tree which is still deterministic.
+*)
+Lemma expand_det_tree {u sP sV sV' A r s} : 
+  check_program sP ->
+    sigma2ctx sP s [::] = Some sV ->
+      det_tree_aux sP sV A Func = ty_ok (Func, sV') ->
+        expand u s A = r ->
+          typ_func (det_tree_aux sP sV' (get_tree r) Func).
+Proof.
+  move=> H ++ <-; clear r.
+  elim: A s sV sV' => //.
+  - move=> p c s sV sV' /=.
+    {
+      rewrite /big_or.
+      case X: F => //=[[sr r]rs]/=.
+      move=> /=.
+      elim: s p c sV sV' => /=.
+      - move=> p c sV sV' []?; subst.
+        rewrite/rev /=.
+        rewrite/check_callable.
+        case X: check_tm => [[[[]d b]|]|]//=.
+        case: d X => //=-[]//=.
+          case: b => //=.
+          case X: get_callable_hd_sig => //[s].
+          case Y: assume_call => //=[sV''] + [?]; subst.
+          rewrite/big_or.
+        
+
+        Search "rev" "nil".
+      clear -H.
+    }
+    move: H.
+    rewrite /check_program.
+    apply is_det_det_tree.
+  - move=> A HA s B HB/=.
+    case X: det_tree_aux => [dA sA].
+    case Y: det_tree_aux => [dB sB].
+    case: ifP => /=.
+      case: dA X => //=; case: dB Y => //= H1 H2 H3 _.
+      case: ifP => DA.
+        rewrite get_tree_Or/= H2/=.
+        move: HB; rewrite H1/=H3 => /(_ erefl).
+        (* TODO: the IH for is not enough generalized... *)
+        admit.
+      move: HA; rewrite H2/= => -/(_ erefl).
+      have:= @expand_has_cut u _ empty H3.
+      case X: expand => //=[s' A'|s' A'|A'|s' A']; 
+      case d: det_tree_aux => //=[s2 sA']; try by move=> []//->/eqP->; rewrite H1//.
+      rewrite is_ko_cutr=> + /eqP?; subst =>/=.
+      have:= @no_alt_cut sP B; rewrite /det_tree.
+      case: det_tree_aux => //= -[]// _ _; case:ifP => //.
+    case: ifP => //; case: dA X => //= X kB cA _.
+    rewrite (is_ko_expand _ kB)/=.
+    case: ifP => dA/=.
+      rewrite X Y cA kB//.
+    move: HA; rewrite X => -/(_ erefl).
+    case e: expand => //=[s' A'|s' A'|A'|s' A']/eqP; try by
+      case: det_tree_aux => -[]//= b _; rewrite Y kB;
+      have:= @no_alt_ko sP B kB;
+      rewrite/det_tree Y => /eqP/=->; case: ifP => //.
+    case: det_tree_aux => -[]//=.
+    have:= @no_alt_cut sP B.
+    rewrite/det_tree.
+    case: det_tree_aux => -[]//= _ _ b _; rewrite is_ko_cutr; case: ifP => //.
+  - move=> A HA B0 HB0 B HB /=.
+    case: ifP => kA.
+      rewrite (is_ko_expand _ kA)/=kA//.
+    move: HA; case dA: det_tree_aux => //=[DA SA] {}HA.
+    (* case: ifP. *)
+    (* move=> /eqP->. *)
+    case dB0: det_tree_aux => //[DB0 SB0]/=.
+    case dB: det_tree_aux => //[DB SB]/=.
+    case: DB0 dB0 => //=; case: DB dB => //= DB DB0 _.
+    move: HA; case e: expand => //=[s' A'|s' A'|A'|s' A']; 
+    rewrite ?eqxx; try case: ifP => //=.
+      case dt: det_tree_aux => //=[dx sx].
+      case: DA dA DB DB0 => //=.
+        move=> ++++/(_ erefl)/eqP?; subst.
+Admitted.
+
+Lemma expand_det_tree {u sP A r} : 
+  check_program sP -> det_tree sP A -> 
+    expand u empty A = r ->
+      det_tree sP (get_tree r).
+Proof.
+
+(* Lemma expand_next_alt {u sP s1 A s2 B} : 
+  check_program sP -> det_tree sP A ->
+    expand u s1 A = Success s2 B -> forall s3, next_alt s3 B = None.
+Proof.
+  move=> H.
+  elim: A s1 B s2 => //.
+  - by move=> /= s1 A s2 _ [_ <-]//.
+  - move=> A HA s B HB s1 C s2/=.
+    move=> /=/andP[fA].
+    case: (ifP  (is_dead _)) => dA.
+      rewrite is_dead_has_cut// => fB.
+      have:= HB s _ _ fB.
+      case X: expand => ///(_ _ _ erefl) H1 [??]; subst => /= s3.
+      rewrite dA H1//.
+    have:= HA s1 _ _ fA.
+    case X: expand => // [s4 A'] /(_ _ _ erefl) H1 + [_<-] s3/=.
+    rewrite (expand_not_dead _ dA X) H1.
+    rewrite success_has_cut ?(expand_solved_same _ X)//.
+    move=>/eqP->.
+    rewrite is_ko_next_alt?if_same//is_ko_cutr//.
+  - move=> A HA B0 _ B HB s1 C s2 /=.
+    move=>/orP[].
+      move=> kA; rewrite is_ko_expand//.
+    move=> /and3P[/orP[/andP[cB0 cB]|fA] fB fB0].
+      case X: expand => // [s3 D].
+      have:= HB s3 _ _ fB.
+      have sbF:= has_cut_success cB.
+      case Y: expand => ///(_ _ _ erefl) H1 [??] s4;subst.
+      have [[]]:= expand_solved_same _ Y; congruence.
+    have:= HA s1 _ _ fA.
+    case X: expand => //[s3 D]/(_ _ _ erefl) H1.
+    have:= HB s3 _ _ fB.
+    case Y: expand => ///(_ _ _ erefl) H2 [??];subst => /= s4.
+    by rewrite H1 H2; rewrite !if_same.
+Qed. *)
+
+Lemma det_tree_next_alt {sP s1 A s2 B}:
+  det_tree sP A -> next_alt s1 A = Some (s2, B) -> det_tree sP B.
+Proof.
+  elim: A s1 B s2 => //.
+  - move=> []//??? _ [_<-]//.
+  - move=>/=??[]//??? _ [_<-]//.
+  - move=> []//??? _ [_<-]//.
+  - move=> A HA s B HB s1 C s2 /=.
+    move=>/andP[fA].
+    case: (ifP (is_dead _)) => dA.
+      rewrite is_dead_has_cut//.
+      move=> fB.
+      have:= HB (Some s) _ _ fB.
+      case X: next_alt => //[[s3 D]] /(_ _ _ erefl) fD[_ <-]/=.
+      rewrite no_alt_dead// is_dead_has_cut// fD.
+    case: ifP => cA.
+      move=> fB.
+      have:= (HA s1 _ _ fA).
+      case X: next_alt => //[[s3 D]|].
+        have cD:= has_cut_next_alt cA X.
+        by move=> /(_ _ _ erefl) fD[_<-]/=; rewrite fD cD fB.
+      move=> _.
+      case: ifP => dB//.
+      have idA := @is_dead_dead A.
+        case Y: next_alt => //[[s3 D]].
+        move=>[_ <-]/=.
+        rewrite no_alt_dead// is_dead_has_cut//.
+        apply: HB fB Y.
+    move=>/eqP->; rewrite (is_ko_next_alt is_ko_cutr) if_same.
+    have:= HA s1 _ _ fA.
+    case: next_alt => // [[s3 D]]/(_ _ _ erefl) fD [_ <-]/=.
+    by rewrite fD cutr2 eqxx no_alt_cut if_same.
+  - move=> A HA B0 HB0 B HB s1 C s2 /=.
+    case: (ifP (is_dead _)) => dA//.
+    move=>/orP[].
+      move=>kA.
+      by rewrite is_ko_failed// is_ko_next_alt//.
+    move=> /and3P[/orP[/andP[cB0 cB]|fA] fB fB0].
+      case: ifP => // fA.
+        case: next_alt => // [[s3 D]]; case: ifP => // _ [_ <-]/=.
+        by rewrite cB0 fB0 orbT.
+      have:= HB s1 _ _ fB.
+      case X: next_alt => // [[s3 D]|].
+        by move=> /(_ _ _ erefl) fD [_ <-]/=; rewrite cB0 (has_cut_next_alt cB X) fD fB0 orbT.
+      move=> _; case: next_alt => // [[s3 D]]; case: ifP => // _ [_ <-]/=.
+      by rewrite cB0 fB0 orbT.
+    case: ifP => // _.
+      have:= HA s1 _ _ fA.
+      case X: next_alt => // [[s3 D]].
+      move=> /(_ _ _ erefl) fD; case: ifP => // _ [_ <-]/=.
+      by rewrite fD orbT fB0 orbT.
+    have:= HB s1 _ _ fB.
+    case: next_alt => // [[s3 D]|].
+      by move=> /(_ _ _ erefl) fD [_ <-]/=; rewrite fA fD fB0 !orbT.
+    move=> _.
+    have:= HA s1 _ _ fA.
+    case X: next_alt => // [[s3 D]].
+    move=> /(_ _ _ erefl) fD; case: ifP => // _ [_ <-]/=.
+    by rewrite fD orbT fB0 orbT.
+Qed.
+
+(* Lemma expand_next_alt_failed {sP A B C s s'}:
+  check_program sP ->
+    det_tree sP A -> expand u s A = Failure B ->
+      forall sN, next_alt sN B = Some (s', C) -> det_tree sP C.
+Proof.
+  move=> Hz.
+  elim: A B C s s' => //.
+  - move=> /=????? []<-//.
+  - move=> /=????? []<-//.
+  - move=> A HA s1 B HB C D s s' /=++sN.
+    move=>/andP[fA].
+    case: (ifP (is_dead _)) => dA.
+      rewrite is_dead_has_cut// => fB.
+      have:= HB _ _ s1 _ fB.
+      case: expand => // E /(_ _ _ _ erefl (Some s1)) + [<-]/=.
+      rewrite dA.
+      case: next_alt => //[[s2 F]] /(_ _ _ erefl) + [_<-]/=.
+      by move=> /= ->; rewrite is_dead_has_cut// no_alt_dead.
+    case: ifP => //.
+      have := HA _ _ s _ fA _ sN.
+      case X: expand => // [E] /(_ _ _ _ erefl) + cA + [?]; subst.
+      rewrite /= (expand_not_dead _ dA X).
+      have:= @expand_has_cut _ s cA; rewrite X/= => -[]// cE.
+      case Y: next_alt => //[[s2 F]|].
+        move=> /(_ _ _ erefl) fF fB [_ <-] /=.
+        have cF:= has_cut_next_alt cE Y.
+        by rewrite fF cF fB.
+      move=>_ fB.
+      case: ifP => // dB.
+      have dDe := @is_dead_dead E.
+        case nB : next_alt => //= [[s2 F]] [_<-]/=.
+        rewrite no_alt_dead// is_dead_has_cut// (det_tree_next_alt fB nB)//.
+    move=> cA /eqP->.
+    have:= HA _ _ s _ fA _ sN.
+    case X: expand => // [E] /(_ _ _ _ erefl) + [<-]/=.
+    have kcB := @is_ko_cutr B.
+    rewrite /= (expand_not_dead _ dA X) (is_ko_next_alt kcB).
+    rewrite if_same.
+    case Y: next_alt => //[[s2 F]].
+    move=> /(_ _ _ erefl) fF [_ <-] /=.
+    by rewrite fF no_alt_cut cutr2 eqxx if_same.
+  - move=> A HA B0 _ B HB C D s s' /= ++sN.
+    move=> /orP[].
+      move=> kA; rewrite is_ko_expand// => -[<-]/=.
+      rewrite is_ko_failed// is_ko_next_alt// if_same//.
+    move=> /and3P[/orP[/andP[cB0 cB]|fA] fB fB0].
+      case X: expand => //[E|s1 E].
+        move=> [<-]/=.
+        case: ifP => // dS.
+        case: ifP => // fS.
+          case nE: next_alt => [[s3 F]|]//.
+          by case: ifP => //FB0 [_<-]/=; rewrite cB0 fB0 orbT.
+        case Y: next_alt => //[[s3 F]|].
+          by move=>[_ <-]/=; rewrite cB0 (has_cut_next_alt cB Y) fB0 (det_tree_next_alt fB Y) orbT.
+        by case: next_alt => // [[s3 F]]; case:ifP=>//_[_<-]/=; rewrite cB0 fB0 orbT.
+      have:= HB _ _ s1 _ fB _ sN.
+      case Z: expand => // [F] /(_ _ _ _ erefl) + [<-]/=.
+      case: ifP => //dE; case:ifP=>FE.
+        move=> _.
+        by case: next_alt => //[[s3 G]]; case:ifP=>//_[_<-]/=; rewrite cB0 fB0 orbT.
+      case Y: next_alt => //[[s3 G]|].
+        move=>/(_ _ _ erefl) nG.
+        have := @expand_has_cut _ s1 cB.
+        rewrite Z/==>-[]//cF.
+        by move=>[_ <-]/=; rewrite cB0 nG fB0 (has_cut_next_alt cF Y) orbT.
+      have [??]:= expand_solved_same _ X; subst => _.
+      case W: next_alt => //[[s3 G]]; case: ifP => // _[_<-]/=.
+      by rewrite cB0 fB0 orbT.
+    have:= HA _ _ s _ fA _ sN.
+    case X: expand => //[E|s1 E].
+      move=> /(_ _ _ _ erefl) + [<-]/=.
+      case: ifP => // dS.
+      case: ifP => //fE.
+        case: next_alt => //[[s4 G]] /(_ _ _ erefl) fG.
+        by case: ifP => // _[_<-]/=; rewrite fB0 fG orbT orbT.
+      case Y: (next_alt sN B) => //[[s4 G]|].
+        by move=> _ [_<-]/=; rewrite (det_tree_next_alt fB Y) fB0 (expand_det_tree Hz fA X) orbT orbT.
+      case: next_alt => //[[s3 G]] /(_ _ _ erefl)fG; case:ifP=>//_[_<-]/=.
+      by rewrite fG fB0 orbT orbT.
+    move=> _.
+    have:= HB _ _ s1 _ fB _ sN.
+    case Z: expand => // [F] /(_ _ _ _ erefl) {}HB [<-]/=.
+    have /= fE := expand_det_tree Hz fA X.
+    case: ifP => //dE; case:ifP=>FE.
+      case W: next_alt => //[[s3 G]]; case:ifP=>//_[_<-]/=.
+      by rewrite fB0 (det_tree_next_alt fE W) orbT orbT.
+    move: HB.
+    case W: next_alt => //[[s3 G]|].
+      move=> /(_ _ _ erefl) fG [_<-]/=; rewrite fG fB0 fE orbT orbT//.
+    case T: next_alt => //[[s3 G]] => _; case:ifP => //[fB01][_<-]/=.
+    by rewrite fB0 (det_tree_next_alt fE T) orbT orbT.
+  Qed. *)
+
+(* Lemma expandedb_next_alt_failed {sP s A B C s' b1}: 
+  check_program sP ->
+    det_tree sP A ->
+      expandedb u s A (Failed B) b1 -> 
+        forall sN, next_alt sN B = Some (s', C) -> det_tree sP C.
+Proof.
+  remember (Failed _) as f eqn:Hf => Hz + H.
+  elim: H B C s' Hf => //; clear -Hz.
+  - move=> s A B HA ? C s' [<-] fA nB.
+    apply: expand_next_alt_failed Hz fA HA nB.
+  - move=> s s' r A B b HA HB IH C D s1 ? fA sN nB; subst.
+    apply: IH erefl (expand_det_tree Hz fA HA) _ nB.
+  - move=> s s' r A B b HA HB IH C D s1 ? fA sN nB; subst.
+    apply: IH erefl (expand_det_tree Hz fA HA) _ nB.
+Qed. *)
+
+Definition is_det A := forall s s' B,
+  run u s A s' B -> forall s2, next_alt s2 B = None.
+
+Lemma runb_next_alt {sP A}: 
+  check_program sP -> 
+    det_tree sP A -> is_det A.
+Proof.
+  rewrite/is_det.
+  move=> H1 H2 s s' B []b H3.
+  elim: H3 H2; clear -H1 => //.
+  - move=> s s' A B C b HA -> fA s2.
+    have H := expandedb_next_alt_done H1 fA HA _.
+    have sB := expanded_Done_success u HA.
+    have//:= next_alt_clean_success sB (H s2).
+  - move=> s s' r A B C D b1 b2 b3 HA HB HC IH ? fA s2; subst.
+    apply: IH.
+    apply: expandedb_next_alt_failed H1 fA HA _ HB.
+Qed.
+
+Lemma main {sP p t}:
+  check_program sP -> callable_is_det sP t -> 
+    is_det ((CallS p t)).
+Proof.
+  move=> H1 fA HA.
+  apply: runb_next_alt H1 _ HA.
+  apply: fA.
+Qed.
+
+Print Assumptions  main.
+
+Section tail_cut.
+
+  Definition tail_cut (r : R) :=
+  match r.(premises) with [::] => false | x :: xs => last x xs == ACut end.
+  
+  Definition AllTailCut := (forall pr : program, all tail_cut (rules pr)).
+
+  Lemma cut_in_prem_tail_cut sP: AllTailCut -> check_program sP.
+  Proof.
+    rewrite /AllTailCut /check_program.
+    rewrite /tail_cut /check_rules.
+    move=> + pr => /(_ pr).
+    remember (rules pr) as RS.
+    apply: sub_all => r; clear.
+    rewrite /check_rule.
+    case X: rcallable_is_det => //=.
+    case: r X => //= hd []//= + l.
+    elim: l => //=.
+    move=> x xs IH []//=; last first.
+      move=> _; apply IH.
+    by move=> H1 H2; rewrite IH//orbT.
+  Qed.
+
+  Lemma tail_cut_is_det sP p t:
+    AllTailCut -> callable_is_det sP t -> is_det ((CallS p t)).
+  Proof.
+    move=> /(cut_in_prem_tail_cut sP).
+    apply main.
+  Qed.
+End tail_cut.
+
+Print Assumptions tail_cut_is_det.
 
 End check.
